add some abbreviations and start Mem version of regular expression algorithm

Validator/Regex/EnterMem.lean
@@ -5,17 +5,31 @@ import Validator.Regex.Enter
 
 namespace Regex
 
-def enterM [DecidableEq σ] [Hashable σ] [Monad m] [MonadState (MemTable (@enter σ)) m]
+def MemTable.enterM [DecidableEq σ] [Hashable σ] [Monad m] [MonadState (MemTable (@enter σ)) m]
   (param: Regex σ): m { res // res = enter param } :=
   MemTable.call enter param
 
+private theorem MemTable.enterM_is_correct [DecidableEq σ] [Hashable σ] (param: Regex σ) (table: (MemTable (@enter σ))):
+  enter param = (StateM.run (s := table) (MemTable.enterM param)).1 := by
+  generalize (StateM.run (MemTable.enterM param) table) = x
+  obtain ⟨⟨res, hres⟩, table'⟩ := x
+  simp only
+  rw [hres]
+
+abbrev enterParam (σ: Type) := Regex σ
+abbrev enterMemTable (σ: Type) [DecidableEq σ] [Hashable σ] := MemTable enter (α := enterParam σ)
+
 instance [DecidableEq σ] [Hashable σ] [Monad m] [MonadState (MemTable (@enter σ)) m]:
   Memoize (α := Regex σ) (β := fun r => Vector σ (symbols r)) enter m where
-  call param := enterM param
+  call param := MemTable.enterM param
 
-private theorem enterM_is_correct [DecidableEq σ] [Hashable σ] (param: Regex σ) (table: (MemTable (@enter σ))):
-  enter param = (StateM.run (s := table) (enterM param)).1 := by
-  generalize (StateM.run (enterM param) table) = x
+abbrev MemoizedEnter (σ: Type) [DecidableEq σ] [Hashable σ] := Memoize (@enter σ) (StateM (enterMemTable σ))
+
+private theorem Memoize.StateM.enterM_is_correct
+  [DecidableEq σ] [Hashable σ] [mementer: MemoizedEnter σ]
+  (param: enterParam σ) (table: enterMemTable σ):
+  enter param = (mementer.call param table).1 := by
+  generalize (mementer.call param table) = x
   obtain ⟨⟨res, hres⟩, table'⟩ := x
   simp only
   rw [hres]
