Validator/Regex/LeaveMem.lean
@@ -9,17 +9,31 @@ namespace Regex
 def leave2 {σ: Type}: (Σ (r: Regex σ), (Vector Bool (symbols r))) → Regex σ
   | ⟨r, bools⟩ => leave r bools
 
-def leaveM {σ: Type} [DecidableEq σ] [Hashable σ] [Monad m] [MonadState (MemTable leave2 (α := (Σ (r: Regex σ), (Vector Bool (symbols r))))) m]
+def MemTable.leaveM {σ: Type} [DecidableEq σ] [Hashable σ] [Monad m] [MonadState (MemTable leave2 (α := (Σ (r: Regex σ), (Vector Bool (symbols r))))) m]
   (param: Σ (r: Regex σ), (Vector Bool (symbols r))): m { res // res = leave2 param } :=
   MemTable.call leave2 param
 
-instance {σ: Type} [DecidableEq σ] [Hashable σ] [Monad m] [MonadState (MemTable leave2 (α := (Σ (r: Regex σ), (Vector Bool (symbols r))))) m]:
-  Memoize (α := (Σ (r: Regex σ), (Vector Bool (symbols r)))) (β := fun _ => Regex σ) leave2 m where
-  call param := leaveM param
-
-private theorem leaveM_is_correct [DecidableEq σ] [Hashable σ] (param: Σ (r: Regex σ), (Vector Bool (symbols r))) (table: (MemTable (@leave2 σ))):
+private theorem MemTable.leaveM_is_correct [DecidableEq σ] [Hashable σ] (param: Σ (r: Regex σ), (Vector Bool (symbols r))) (table: (MemTable (@leave2 σ))):
   leave2 param = (StateM.run (s := table) (leaveM param)).1 := by
   generalize (StateM.run (leaveM param) table) = x
+  obtain ⟨⟨res, hres⟩, table'⟩ := x
+  simp only
+  rw [hres]
+
+abbrev leaveParam (σ: Type) := Σ (r: Regex σ), (Vector Bool (symbols r))
+abbrev leaveMemTable (σ: Type) [DecidableEq σ] [Hashable σ] := MemTable leave2 (α := leaveParam σ)
+
+instance {σ: Type} [DecidableEq σ] [Hashable σ] [Monad m] [MonadState (leaveMemTable σ) m]:
+  Memoize (α := leaveParam σ) (β := fun _ => Regex σ) leave2 m where
+  call param := MemTable.leaveM param
+
+abbrev MemoizedLeave (σ: Type) [DecidableEq σ] [Hashable σ] := Memoize (@leave2 σ) (StateM (leaveMemTable σ))
+
+private theorem Memoize.StateM.leaveM_is_correct
+  [DecidableEq σ] [Hashable σ] [memleave: MemoizedLeave σ]
+  (param: leaveParam σ) (table: leaveMemTable σ):
+  leave2 param = (memleave.call param table).1 := by
+  generalize (memleave.call param table) = x
   obtain ⟨⟨res, hres⟩, table'⟩ := x
   simp only
   rw [hres]
