Validator/Regex/Memoize.lean
@@ -1,0 +1,17 @@
+import Validator.Std.Vec
+import Validator.Std.Memoize
+
+import Validator.Regex.EnterMem
+import Validator.Regex.Drawer
+import Validator.Regex.Lang
+import Validator.Regex.Leave
+import Validator.Regex.Num
+import Validator.Regex.Regex
+
+def Regex.Mem.derive
+  [DecidableEq σ] [Hashable σ]
+  [mementer: MemoizedEnter σ]
+  (Φ: σ → Bool) (r: Regex σ): StateM (MemTable (@enter σ)) (Regex σ) := do
+  let ⟨ss, _⟩ <- mementer.call r
+  let bools := Vector.map Φ ss
+  return leave r bools
